

% trial .tex file %
\documentclass[9pt]{article}  % specifies document class (article) and point size (10pt)
\usepackage{graphicx}
\usepackage{polski}
\usepackage[utf8]{inputenc}
\usepackage{sidecap}
\usepackage{wrapfig}
\usepackage{subfig}
\usepackage{amsmath}
\usepackage{float}
\usepackage{enumerate}
\usepackage{listings}
\usepackage{listings}
\usepackage{color}

\definecolor{dkgreen}{rgb}{0,0.6,0}
\definecolor{gray}{rgb}{0.5,0.5,0.5}
\definecolor{mauve}{rgb}{0.58,0,0.82}

\lstset{frame=tb,
  language=R,
  aboveskip=3mm,
  belowskip=3mm,
  showstringspaces=false,
  columns=flexible,
  basicstyle={\small\ttfamily},
  numbers=none,
  numberstyle=\tiny\color{gray},
  keywordstyle=\color{blue},
  commentstyle=\color{dkgreen},
  stringstyle=\color{mauve},
  breaklines=true,
  breakatwhitespace=true,
  tabsize=3
}


\begin{document}               % starts document

\section{Regresja liniowa}

  $Y_i = \beta_0 + \beta_1 X_i + \xi_i$, $\beta_0$ $\beta_1$ $\xi_i \sim N \left(0, \sigma^2 \right)$ $E(Y_i | X_i) = \beta_0 + \beta_1 X_i$, $Var(Y_i | X_i) = \sigma^2$
  
  
\section{Estymacja}


  $\hat{Y} = b_0 + b_1 X_i$, $e_i = Y_i - \hat{Y} = Y_i - (b_0 + b_1 X_i)$
  $
  b_1 = \frac{\sum{\left(X_i - \bar{X} \right) \left( Y_i - \bar{Y} \right) } }{\sum{\left(X_i - \bar{X} \right) ^2 } }
  $, $
  b_0 = \bar{Y} - b_1 \bar{X}
  $
  
  
    $$ s^2 = \frac{ \sum{ \left( Y_i - \hat{Y_i} \right)^2 } } { n-2 }  = \frac{ \sum{e^2_i}  }{n-2} = \frac{SSE}{dfE} = MSE$$
  
  
  
  \section{Przedziały ufności}
  
    \subsection{ Dla $\beta_1$ }
    
    $b_1 \sim N(\beta_1, \sigma^2(b_1)) $, 
    $\sigma^2(b_1) = \frac{\sigma^2}{\sum{\left(X_i - \bar{X}\right)^2 }}$, 
    $ t = \frac{ \left(b_1 - \beta_1 \right) }{ s(b_1) } \sim t(n-2)$, 
    $s^2(b_1) = \frac{s^2}{\sum{\left(X_i - \bar{X}\right)^2}}$, 


    $ b_1 \pm t_c s(b_1)$, 
    $ t_c = (1-\alpha /2, n-2)$


    $P(|z| \ge |t|)$ , $z \sim t(n-2)$ \newline
    
    
    \subsection{ Dla $\beta_0$ }
    
      $b_1 \sim N(\beta_0, \sigma^2(b_0)) $, 
    
    $\sigma^2(b_0) = \sigma^2 \left[ \frac{1}{n} + \frac{\bar{X}^2}{\sum{\left(X_i - \bar{X}\right)^2 }}  \right]$, 

  $t = \frac{b_0+\beta_0}{s(b_0)} \sim t(n-2)$
  
      $s^2(b_0) = s^2 \left[ \frac{1}{n} + \frac{\bar{X}^2}{\sum{\left(X_i - \bar{X}\right)^2 }}  \right]$, 

    $ b_0 \pm t_c s(b_0)$, 
    $ t_c = (1-\alpha /2, n-2)$, 


      $t = \frac{b_0+\beta_{00}}{s(b_0)}$, 
    $P(|z| \ge |t|)$, $$z \sim t(n-2)$

    

    
    
\section{Moc}

    
    $ t = \frac{ b_1 }{ s(b_1) } \sim t(n-2,\delta)$,
    $\delta = \frac{\beta_1}{\sigma(b_1)}$,

    $b_1 \sim N(\beta_1, \sigma_2(b_1)) $,

    $\sigma^2(b_1) = \frac{\sigma^2}{\sum{\left(X_i - \bar{X}\right)^2 }}$,


  
\section{Estymacja średniej}

  $E(Y_h) = \mu_h = \beta_0 + \beta_1 X_h  $,
  
  $ \hat{\mu}_h = b_0 + b_1 X_h $,
  
  $ \hat{\mu}_h \sim N(\mu_h, \sigma^2) $,
  
  $\sigma^2 (\hat{\mu}_h) = \sigma^2 \left[  \frac{1}{n} + \frac{(X_h-\bar{X})^2 }{\sum{(X_i-\bar{X})^2} }   \right]$,
  
  
    
  $s^2 (\hat{\mu}_h) = s^2 \left[  \frac{1}{n} + \frac{(X_h-\bar{X})^2 }{\sum{(X_i-\bar{X})^2} }   \right]$,


  $ \frac{ \hat{\mu}_h - E(Y_h) }{s(\hat{\mu}_h) } \sim t(n-2) $



    $\hat{\mu}_h \pm t_c s(\hat{\mu}_h) $
    
    
    
\section{Prognoza}

  $Y_h = \beta_0 + \beta_1 X_h + \xi_h$,
  
  
    $s^2 (pred) = s^2 \left[ 1+ \frac{1}{n} + \frac{(X_h-\bar{X})^2 }{\sum{(X_i-\bar{X})^2} }   \right]$,
    
    $ \frac{Y_h -  \hat{\mu}_h }{s(pred)} \sim t(n-2)$,


    $\hat{\mu}_h \pm t_c s(pred) $
    
\section{ANOVA}


  
  $ SST = \sum(Y_i - \bar{Y})^2  $,
  $dfT = n-1$,
  $ MST = \frac{SST}{dfT}$
  
  

  
  $ SSM = \sum(\hat{Y}_i - \bar{Y})^2  $,
  $dfM = 1$,
  $ MSM = \frac{SSM}{dfM}$
  

  
    $ SSE = \sum(Y_i - \hat{Y}_i)^2  $,
  $dfE = n-2$,
  $ MSE = \frac{SSE}{dfE}$
  
  

  
  $F = \frac{MSM}{MSE} \sim F(dfM, dfE) = F(1, n-2)$
  
  
  \section{Porównywanie modeli}
  
  $$F = \frac{ \frac{ SSE(R) - SSE(F)  }{ dfE(R) - dfE(F)  } }{ MSE(F)}$$
  $SSE(R) = \sum{\left( Y_i - b_0 \right)^2} = \sum{\left( Y_i - \bar{Y} \right)^2} = SST$
  $SSE(F) = SSE$
  $dfE(R) = n-1$
  $dfE(F) = n-2$
  $$r^2 = SSM/SST = 1-SSE/SST$$
  
  

\end{document}  







